michael_formal/Nondeterministic_EFSM.thy
@@ -1,0 +1,34 @@
+theory Nondeterministic_EFSM
+imports EFSM
+begin
+
+definition nondeterministic_step :: "transition_matrix \<Rightarrow> nat \<Rightarrow> datastate \<Rightarrow> label \<Rightarrow> inputs \<Rightarrow> (transition \<times> nat \<times> outputs \<times> datastate) option" where
+"nondeterministic_step e s r l i = (
+  if \<exists>x. x |\<in>| (possible_steps e s r l i) then (
+    let (s', t) =  (Eps (\<lambda>x. x |\<in>| (possible_steps e s r l i))) in
+    Some (t, s', (apply_outputs (Outputs t) (join_ir i r)), (apply_updates (Updates t) (join_ir i r) r)))
+  else None)"
+
+primrec nondeterministic_observe_all :: "transition_matrix \<Rightarrow> nat \<Rightarrow> datastate \<Rightarrow> trace \<Rightarrow> (transition \<times> nat \<times> outputs \<times> datastate) list" where
+  "nondeterministic_observe_all _ _ _ [] = []" |
+  "nondeterministic_observe_all e s r (h#t) =
+    (case (nondeterministic_step e s r (fst h) (snd h)) of
+      (Some (transition, s', outputs, updated)) \<Rightarrow> (((transition, s', outputs, updated)#(observe_all e s' updated t))) |
+      _ \<Rightarrow> []
+    )"
+
+definition nondeterministic_observe_trace :: "transition_matrix \<Rightarrow> nat \<Rightarrow> datastate \<Rightarrow> trace \<Rightarrow> observation" where
+  "nondeterministic_observe_trace e s r t \<equiv> map (\<lambda>(t,x,y,z). y) (nondeterministic_observe_all e s r t)"
+
+inductive nondeterministic_simulates_trace :: "transition_matrix \<Rightarrow> transition_matrix \<Rightarrow> nat \<Rightarrow> nat \<Rightarrow> datastate \<Rightarrow> datastate \<Rightarrow> trace \<Rightarrow> bool" where
+  base: "nondeterministic_simulates_trace e1 e2 s1 s2 d1 d2 []" |
+  step_some: "nondeterministic_step e1 s1 d1 (fst h) (snd h) = Some (tr1, s1', p', d1') \<Longrightarrow>
+              \<exists>tr2. nondeterministic_step e2 s2 d2 (fst h) (snd h) = Some (tr2, s2', p', d2') \<and>
+              nondeterministic_simulates_trace e1 e2 s1' s2' d1' d2' t \<Longrightarrow>
+              nondeterministic_simulates_trace e1 e2 s1 s2 d1 d2 (h#t)" |
+  step_none: "nondeterministic_step e1 s1 d1 (fst h) (snd h) = None \<Longrightarrow> nondeterministic_simulates_trace e1 e2 s1 s2 d1 d2 (h#t)"
+
+definition nondeterministic_simulates :: "transition_matrix \<Rightarrow> transition_matrix \<Rightarrow> bool" where
+  "nondeterministic_simulates m1 m2 = (\<forall>t. nondeterministic_simulates_trace m1 m2 0 0 <> <> t)"
+
+end
