michael_formal/not4afp/Paper_Example.thy
@@ -1,0 +1,310 @@
+theory Paper_Example
+imports Inference
+begin
+
+definition select :: transition where
+  "select = \<lparr>
+              Label = ''select'',
+              Arity = 1,
+              Guard = [],
+              Outputs = [],
+              Updates = [(R 1, V (I 1))]
+            \<rparr>"
+
+definition coin50 :: transition where
+  "coin50 = \<lparr>
+              Label = ''coin'',
+              Arity = 1,
+              Guard = [gexp.Eq (V (I 1)) (L (Num 50))],
+              Outputs = [L (Num 50)],
+              Updates = [(R 2, L (Num 50))]
+            \<rparr>"
+
+definition coin :: transition where
+  "coin = \<lparr>
+              Label = ''coin'',
+              Arity = 1,
+              Guard = [],
+              Outputs = [Plus (V (R 2)) (V (I 1))],
+              Updates = [(R 2, Plus (V (R 2)) (V (I 1)))]
+            \<rparr>"
+
+definition vend_fail :: transition where
+  "vend_fail = \<lparr>
+              Label = ''vend'',
+              Arity = 0,
+              Guard = [GExp.Lt (V (R 2)) (L (Num 100))],
+              Outputs = [],
+              Updates = []
+            \<rparr>"
+
+definition vend_success :: transition where
+  "vend_success = \<lparr>
+              Label = ''vend'',
+              Arity = 0,
+              Guard = [GExp.Ge (V (R 2)) (L (Num 100))],
+              Outputs = [(V (R 1))],
+              Updates = []
+            \<rparr>"
+
+definition select_update :: transition where
+  "select_update = \<lparr>
+              Label = ''select'',
+              Arity = 1,
+              Guard = [],
+              Outputs = [],
+              Updates = [(R 1, V (I 1)), (R 2, L (Num 0))]
+            \<rparr>"
+
+declare One_nat_def [simp del]
+
+definition drinks_before :: transition_matrix where
+  "drinks_before = {|((0, 1), select), ((1, 2), coin50), ((2, 2), coin), ((2, 2), vend_fail), ((2, 3), vend_success)|}"
+
+definition drinks_after :: transition_matrix where
+  "drinks_after = {|((0, 1), select_update), ((1, 1), coin), ((1, 1), vend_fail), ((1, 2), vend_success)|}"
+
+definition merge_1_2 :: transition_matrix where
+  "merge_1_2 = {|((0, 1), select), ((1, 1), coin50), ((1, 1), coin), ((1, 1), vend_fail), ((1, 3), vend_success)|}"
+
+lemma merge_1_2: "merge_states 1 2 drinks_before = merge_1_2"
+  by (simp add: merge_states_def drinks_before_def merge_1_2_def merge_states_aux_def)
+
+definition merge_1_2_update :: transition_matrix where
+  "merge_1_2_update = {|((0, 1), select_update), ((1, 1), coin50), ((1, 1), coin), ((1, 1), vend_fail), ((1, 3), vend_success)|}"
+
+lemmas transitions = select_def coin_def coin50_def vend_fail_def vend_success_def select_update_def
+
+lemma possible_steps_drinks_before_select: "length b = 1 \<Longrightarrow> possible_steps drinks_before 0 r ''select'' b = {|(1, select)|}"
+proof-
+  assume premise: "length b = 1"
+  have set_filter: "(Set.filter
+       (\<lambda>((origin, dest), t).
+           origin = 0 \<and>
+           Label t = ''select'' \<and> length b = Arity t \<and> apply_guards (Guard t) (case_vname (\<lambda>n. input2state b 1 (I n)) (\<lambda>n. r (R n))))
+       (fset drinks_before)) = {((0, 1), select)}"
+    apply (simp add: Set.filter_def drinks_before_def)
+    apply safe
+    by (simp_all add: transitions premise)
+  show ?thesis
+    by (simp add: possible_steps_def ffilter_def set_filter)
+qed
+
+lemma possible_steps_merge_1_2_select: "length b = 1 \<Longrightarrow> possible_steps merge_1_2 0 r ''select'' b = {|(1, select)|}"
+proof-
+  assume premise: "length b = 1"
+  have set_filter: "(Set.filter
+       (\<lambda>((origin, dest), t).
+           origin = 0 \<and>
+           Label t = ''select'' \<and> length b = Arity t \<and> apply_guards (Guard t) (case_vname (\<lambda>n. input2state b 1 (I n)) (\<lambda>n. r (R n))))
+       (fset merge_1_2)) =
+    {((0, 1), select)}"
+    apply (simp add: merge_1_2_def Set.filter_def)
+    apply safe
+    by (simp_all add: transitions premise)
+  show ?thesis
+    by (simp add: possible_steps_def ffilter_def set_filter)
+qed
+
+lemma possible_steps_merge_1_2_update_select: "length b = 1 \<Longrightarrow> possible_steps merge_1_2_update 0 r ''select'' b = {|(1, select_update)|}"
+proof-
+  assume premise: "length b = 1"
+  have set_filter: "(Set.filter
+       (\<lambda>((origin, dest), t).
+           origin = 0 \<and>
+           Label t = ''select'' \<and> length b = Arity t \<and> apply_guards (Guard t) (case_vname (\<lambda>n. input2state b 1 (I n)) (\<lambda>n. r (R n))))
+       (fset merge_1_2_update)) =
+    {((0, 1), select_update)}"
+    apply (simp add: Set.filter_def merge_1_2_update_def)
+    apply safe
+    by (simp_all add: transitions premise)
+  show ?thesis
+    by (simp add: possible_steps_def ffilter_def set_filter)
+qed
+
+lemma drinks_before_step_0_invalid: "\<not> (aa = ''select'' \<and> length b = 1) \<Longrightarrow>
+        nondeterministic_step drinks_before 0 Map.empty aa b = None"
+proof-
+  assume premise: "\<not> (aa = ''select'' \<and> length b = 1)"
+  have set_filter: "(Set.filter
+           (\<lambda>((origin, dest), t).
+               origin = 0 \<and> Label t = aa \<and> length b = Arity t \<and> apply_guards (Guard t) (case_vname (\<lambda>n. input2state b 1 (I n)) Map.empty))
+           (fset drinks_before)) = {}"
+    apply (simp add: Set.filter_def drinks_before_def)
+    apply safe
+    using premise
+    by (simp_all add: transitions)
+  show ?thesis
+    apply (simp add: nondeterministic_step_def possible_steps_def ffilter_def set_filter)
+    using bot_fset.abs_eq by auto
+qed
+
+lemma possible_steps_drinks_before_coin_50: "possible_steps drinks_before 1 r ''coin'' [Num 50] = {|(2, coin50)|}"
+proof-
+  have set_filter: "(Set.filter
+       (\<lambda>((origin, dest), t).
+           origin = 1 \<and>
+           Label t = ''coin'' \<and> Suc 0 = Arity t \<and> apply_guards (Guard t) (case_vname (\<lambda>n. input2state [Num 50] 1 (I n)) (\<lambda>n. r (R n))))
+       (fset drinks_before)) =
+    {((1, 2), coin50)}"
+    apply (simp add: drinks_before_def Set.filter_def)
+    apply safe
+    by (simp_all add: transitions)
+  have abs_fset: "Abs_fset {((1, 1), coin50), ((1, 1), coin)} = {|((1, 1), coin50), ((1, 1), coin)|}"
+    by (metis finsert.rep_eq fset_inverse fset_simps(1))
+   show ?thesis
+     by (simp add: possible_steps_def ffilter_def set_filter abs_fset)
+ qed
+
+lemma drinks_before_1_invalid: "\<not>(aa = ''coin'' \<and> b = [Num 50]) \<Longrightarrow> nondeterministic_step drinks_before 1 r aa b = None"
+proof-
+  assume premise: "\<not>(aa = ''coin'' \<and> b = [Num 50])"
+  have set_filter: "(Set.filter
+           (\<lambda>((origin, dest), t).
+               origin = 1 \<and>
+               Label t = aa \<and> length b = Arity t \<and> apply_guards (Guard t) (case_vname (\<lambda>n. input2state b 1 (I n)) (\<lambda>n. r (R n))))
+           (fset drinks_before)) = {}"
+    using premise
+    apply (simp add: drinks_before_def Set.filter_def coin50_def)
+    by (metis One_nat_def input2state.simps(2) length_0_conv length_Suc_conv option.inject)
+  show ?thesis
+    apply (simp add: nondeterministic_step_def possible_steps_def ffilter_def set_filter)
+    using bot_fset.abs_eq by auto
+qed
+
+lemma merge_1_2_invalid_coin_input: "aa = ''coin'' \<Longrightarrow> length b \<noteq> 1 \<Longrightarrow> nondeterministic_step merge_1_2 1 <R 1 := d> ''coin'' b = None"
+proof-
+  assume premise1: "aa = ''coin''"
+  assume premise2: "length b \<noteq> 1"
+  have set_filter: "(Set.filter
+           (\<lambda>((origin, dest), t).
+               origin = 1 \<and>
+               Label t = ''coin'' \<and>
+               length b = Arity t \<and> apply_guards (Guard t) (case_vname (\<lambda>n. input2state b 1 (I n)) (\<lambda>n. if n = 1 then Some d else None)))
+           (fset merge_1_2)) = {}"
+    using premise1 premise2
+    apply (simp add: merge_1_2_def Set.filter_def)
+    apply safe
+    by (simp_all add: transitions)
+  show ?thesis
+    apply (simp add: nondeterministic_step_def possible_steps_def ffilter_def set_filter)
+    using bot_fset_def by force
+qed
+
+lemma merge_1_2_possible_steps_coin_not_50: "aa = ''coin'' \<Longrightarrow>
+    length b = 1 \<Longrightarrow>
+    b \<noteq> [Num 50] \<Longrightarrow>
+    possible_steps merge_1_2 1 <R 1 := d> ''coin'' b = {|(1, coin)|}"
+proof-
+  assume premise1: "aa = ''coin''"
+  assume premise2: "length b = 1"
+  assume premise3: "b \<noteq> [Num 50]"
+  have set_filter: "(Set.filter
+       (\<lambda>((origin, dest), t).
+           origin = 1 \<and>
+           Label t = ''coin'' \<and> length b = Arity t \<and> apply_guards (Guard t) (case_vname (\<lambda>n. input2state b 1 (I n)) (\<lambda>n. <R 1 := d> (R n))))
+       (fset merge_1_2)) = {((1, 1), coin)}"
+    using premise1 premise2 premise3
+    apply (simp add: merge_1_2_def Set.filter_def)
+    apply safe
+           apply (simp_all add: transitions)
+    by (metis One_nat_def input2state.simps(2) length_0_conv length_Suc_conv option.inject)
+  show ?thesis
+    by (simp add: possible_steps_def ffilter_def set_filter)
+qed
+
+lemma merge_1_2_update_possible_steps_coin_50: "possible_steps merge_1_2_update 1 <R 1 := d, R 2 := Num n> ''coin'' [Num 50] = {|(1, coin50), (1, coin)|}"
+proof-
+  have set_filter: "(Set.filter
+       (\<lambda>((origin, dest), t).
+           origin = 1 \<and>
+           Label t = ''coin'' \<and>
+           Suc 0 = Arity t \<and> apply_guards (Guard t) (case_vname (\<lambda>n. input2state [Num 50] 1 (I n)) (\<lambda>na. <R 1 := d, R 2 := Num n> (R na))))
+       (fset merge_1_2_update)) = {((1, 1), coin), ((1, 1), coin50)}"
+    apply (simp add: Set.filter_def merge_1_2_update_def)
+    apply safe
+    by (simp_all add: transitions)
+  have abs_fset: "Abs_fset {((1, 1), coin), ((1, 1), coin50)} = {|((1, 1), coin), ((1, 1), coin50)|}"
+    by (metis finsert.rep_eq fset_inverse fset_simps(1))
+  show ?thesis
+    apply (simp add: possible_steps_def ffilter_def set_filter abs_fset)
+    by auto
+qed
+
+lemma simulation_1_1: "nondeterministic_simulates_trace drinks_before merge_1_2_update 1 1 <R 1 := d> <R 1 := d, R 2 := Num 0> ((aa, b) # list)"
+proof-
+  have choice_coin50_coin: "(\<exists>a b. a = 1 \<and> b = coin50 \<or> a = 1 \<and> b = coin)"
+    by auto
+  have abs_fset_empty: "Abs_fset {} = {||}"
+    by (simp add: bot_fset_def)
+  have set_filter: "\<forall>b d. (Set.filter
+            (\<lambda>((origin, dest), t).
+                origin = 1 \<and>
+                Label t = ''vend'' \<and>
+                length b = Arity t \<and> apply_guards (Guard t) (case_vname (\<lambda>n. input2state b 1 (I n)) (\<lambda>n. if n = 1 then Some d else None)))
+            (fset merge_1_2)) = {}"
+    apply (simp add: merge_1_2_def Set.filter_def)
+    apply safe
+    by (simp_all add: transitions)
+  show ?thesis
+    apply (case_tac "aa = ''coin'' \<and> b = [Num 50]")
+     prefer 2
+     apply (rule nondeterministic_simulates_trace.step_none)
+      apply (simp add: drinks_before_1_invalid)
+    
+    apply (rule nondeterministic_simulates_trace.step_some)
+     apply (simp add: nondeterministic_step_def possible_steps_drinks_before_coin_50)
+    apply (rule_tac x=coin50 in exI)
+    apply (simp add: nondeterministic_step_def merge_1_2_update_possible_steps_coin_50 choice_coin50_coin)
+    apply safe
+
+    sorry
+qed
+
+lemma simulation_0_0: "nondeterministic_simulates_trace drinks_before merge_1_2_update 0 0 Map.empty Map.empty ((aa, b) # t)"
+proof-
+  have select_updates: "length b = 1 \<Longrightarrow> (\<lambda>x. if x = R 1 then aval (snd (R 1, V (I 1))) (case_vname (\<lambda>n. input2state b 1 (I n)) Map.empty)
+          else EFSM.apply_updates [] (case_vname (\<lambda>n. input2state b 1 (I n)) Map.empty) Map.empty x) = <R 1 := hd b>"
+    apply (rule ext)
+    by (simp add: hd_input2state select_def)
+  have select_update_updates: "length b = 1 \<Longrightarrow> (\<lambda>x. if x = R 1 then aval (snd (R 1, V (I 1))) (case_vname (\<lambda>n. input2state b 1 (I n)) Map.empty)
+          else EFSM.apply_updates [(R 2, L (Num 0))] (case_vname (\<lambda>n. input2state b 1 (I n)) Map.empty) Map.empty x) = <R 1 := hd b, R 2 := Num 0>"
+    apply (rule ext)
+    by (simp add: hd_input2state)
+  show ?thesis
+  apply (case_tac "aa = ''select'' \<and> length b = 1")
+   apply (rule nondeterministic_simulates_trace.step_some)
+     apply (simp add: nondeterministic_step_def possible_steps_drinks_before_select)
+    apply (simp add: nondeterministic_step_def possible_steps_merge_1_2_update_select transitions)
+   defer
+   apply (rule nondeterministic_simulates_trace.step_none)
+     apply (simp add: drinks_before_step_0_invalid)
+    apply safe
+      apply simp
+     apply simp
+    apply (simp add: select_updates select_update_updates)
+    apply (case_tac t)
+     apply (simp add: nondeterministic_simulates_trace.base)
+    apply (case_tac a)
+    by (simp add: simulation_1_1)
+qed
+
+lemma simulation_aux: "nondeterministic_simulates_trace merge_1_2 merge_1_2_update 0 0 Map.empty Map.empty t"
+proof (induct t)
+case Nil
+  then show ?case
+    by (simp add: nondeterministic_simulates_trace.base)
+next
+  case (Cons a t)
+  then show ?case
+    apply (case_tac a)
+    by (simp add: simulation_0_0)
+qed
+
+lemma simulation: "nondeterministic_simulates merge_1_2 merge_1_2_update"
+  apply (simp add:nondeterministic_simulates_def)
+  apply (rule allI)
+  by (simp add: simulation_aux)
+
+
+end
